Using size_t everywhere, second attempt? SHMEM passes and extracts

src/lib/poly/gemm/Kuiper.Poly.GEMM.SHMem.fst
@@ -70,25 +70,29 @@ let kpre1
   (comb : binop et)
   (#mrows #mshared #mcols : sz)
   (tile : valid_tile)
-  (#lA : mlayout (mrows   * tile) (mshared * tile))
-  (#lB : mlayout (mshared * tile) (mcols   * tile))
-  (#lC : mlayout (mrows   * tile) (mcols   * tile))
+  (#_ : squash (SZ.fits (SZ.v mrows   * SZ.v tile)))
+  (#_ : squash (SZ.fits (SZ.v mshared * SZ.v tile)))
+  (#_ : squash (SZ.fits (SZ.v mcols   * SZ.v tile)))
+  (#_ : squash (SZ.fits (SZ.v mrows   * SZ.v mcols)))
+  (#lA : mlayout (mrows   *^ tile) (mshared *^ tile))
+  (#lB : mlayout (mshared *^ tile) (mcols   *^ tile))
+  (#lC : mlayout (mrows   *^ tile) (mcols   *^ tile))
   (gA : gpu_matrix et lA)
   (gB : gpu_matrix et lB)
   (gC : gpu_matrix et lC)
   (eA eB : ematrix _ _ _)
   (fA fB : perm)
-  (bid : natlt (mrows * mcols))
-  (tid : natlt (tile * tile))
+  (bid : szlt (mrows *^ mcols))
+  (tid : szlt (tile *^ tile))
   : slprop
   =
   (gA |-> Frac (fA /. mlayout_size lC) eA) **
   (gB |-> Frac (fB /. mlayout_size lC) eB) **
   (exists* v.
     gpu_matrix_pts_to_cell
-      (gpu_matrix_subtile gC tile tile (bid / mcols) (bid % mcols))
+      (gpu_matrix_subtile gC tile tile (bid /^ mcols) (bid %^ mcols))
       #1.0R
-      (tid / tile) (tid % tile) v)
+      (tid /^ tile) (tid %^ tile) v)
 
 (* NO FUNCTIONAL SPEC RIGHT NOW *)
 unfold
@@ -97,33 +101,37 @@ let kpost1
   (comb : binop et)
   (#mrows #mshared #mcols : sz)
   (tile : valid_tile)
-  (#lA : mlayout (mrows   * tile) (mshared * tile))
-  (#lB : mlayout (mshared * tile) (mcols   * tile))
-  (#lC : mlayout (mrows   * tile) (mcols   * tile))
+  (#_ : squash (SZ.fits (SZ.v mrows   * SZ.v tile)))
+  (#_ : squash (SZ.fits (SZ.v mshared * SZ.v tile)))
+  (#_ : squash (SZ.fits (SZ.v mcols   * SZ.v tile)))
+  (#_ : squash (SZ.fits (SZ.v mrows   * SZ.v mcols)))
+  (#lA : mlayout (mrows   *^ tile) (mshared *^ tile))
+  (#lB : mlayout (mshared *^ tile) (mcols   *^ tile))
+  (#lC : mlayout (mrows   *^ tile) (mcols   *^ tile))
   (gA : gpu_matrix et lA)
   (gB : gpu_matrix et lB)
   (gC : gpu_matrix et lC)
   (eA eB : ematrix _ _ _)
   (fA fB : perm)
-  (bid : natlt (mrows * mcols))
-  (tid : natlt (tile * tile))
+  (bid : szlt (mrows *^ mcols))
+  (tid : szlt (tile *^ tile))
   : slprop
   =
   (gA |-> Frac (fA /. mlayout_size lC) eA) **
   (gB |-> Frac (fB /. mlayout_size lC) eB) **
   (exists* v.
     gpu_matrix_pts_to_cell
-      (gpu_matrix_subtile gC tile tile (bid / mcols) (bid % mcols))
+      (gpu_matrix_subtile gC tile tile (bid /^ mcols) (bid %^ mcols))
       #1.0R
-      (tid / tile) (tid % tile) v)
+      (tid /^ tile) (tid %^ tile) v)
 
 let barrier_tok
   (#et : Type0)
   (tile : valid_tile)
   (l1 l2 : full_mlayout tile tile)
-  (ar1 ar2 : gpu_array et (tile * tile))
+  (ar1 ar2 : gpu_array et (tile *^ tile))
   (it : nat)
-  (tid : natlt (tile *^ tile))
+  (tid : szlt (tile *^ tile))
   : slprop
   =
   B.barrier_tok
@@ -138,9 +146,13 @@ let kpre
   (#mrows #mshared #mcols : sz)
   (tile : valid_tile)
   (slA slB : full_mlayout tile tile) // shmem layouts
-  (#lA : mlayout (mrows   * tile) (mshared * tile))
-  (#lB : mlayout (mshared * tile) (mcols   * tile))
-  (#lC : mlayout (mrows   * tile) (mcols   * tile))
+  (#_ : squash (SZ.fits (SZ.v mrows   * SZ.v tile)))
+  (#_ : squash (SZ.fits (SZ.v mshared * SZ.v tile)))
+  (#_ : squash (SZ.fits (SZ.v mcols   * SZ.v tile)))
+  (#_ : squash (SZ.fits (SZ.v mrows   * SZ.v mcols)))
+  (#lA : mlayout (mrows   *^ tile) (mshared *^ tile))
+  (#lB : mlayout (mshared *^ tile) (mcols   *^ tile))
+  (#lC : mlayout (mrows   *^ tile) (mcols   *^ tile))
   (gA : gpu_matrix et lA)
   (gB : gpu_matrix et lB)
   (gC : gpu_matrix et lC)
@@ -149,14 +161,14 @@ let kpre
   (sh : c_shmems (shmems_desc et tile))
   // ((ar, ()) : c_shmems (shmems_desc et tile))
   // ^ will this work nicely?
-  (bid : natlt (mrows * mcols))
-  (tid : natlt (tile * tile))
+  (bid : szlt (mrows *^ mcols))
+  (tid : szlt (tile *^ tile))
   : slprop
   =
   kpre1 comb tile gA gB gC eA eB fA fB bid tid **
   (exists* x. gpu_pts_to_array (fst sh) #(1.0R /. (tile * tile)) x) **
   (exists* x. gpu_pts_to_array (fst (snd sh)) #(1.0R /. (tile * tile)) x) **
-  barrier_tok tile slA slB (fst sh) (fst (snd sh)) 0 tid
+  barrier_tok tile slA slB (fst sh) (fst (snd sh)) 0sz tid
 
 
 unfold
@@ -166,9 +178,14 @@ let kpost
   (#mrows #mshared #mcols : sz)
   (tile : valid_tile)
   (slA slB : full_mlayout tile tile) // shmem layouts
-  (#lA : mlayout (mrows   * tile) (mshared * tile))
-  (#lB : mlayout (mshared * tile) (mcols   * tile))
-  (#lC : mlayout (mrows   * tile) (mcols   * tile))
+  (#_ : squash (SZ.fits (SZ.v mrows   * SZ.v tile)))
+  (#_ : squash (SZ.fits (SZ.v mshared * SZ.v tile)))
+  (#_ : squash (SZ.fits (SZ.v mcols   * SZ.v tile)))
+  (#_ : squash (SZ.fits (SZ.v mrows   * SZ.v mcols)))
+  (#_ : squash (SZ.fits (2 * SZ.v mshared)))
+  (#lA : mlayout (mrows   *^ tile) (mshared *^ tile))
+  (#lB : mlayout (mshared *^ tile) (mcols   *^ tile))
+  (#lC : mlayout (mrows   *^ tile) (mcols   *^ tile))
   (gA : gpu_matrix et lA)
   (gB : gpu_matrix et lB)
   (gC : gpu_matrix et lC)
@@ -176,14 +193,14 @@ let kpost
   (fA fB : perm)
   (sh : c_shmems (shmems_desc et tile))
   // (ar : gpu_array et (2 * tile * tile))
-  (bid : natlt (mrows * mcols))
-  (tid : natlt (tile * tile))
+  (bid : szlt (mrows *^ mcols))
+  (tid : szlt (tile *^ tile))
   : slprop
   =
-  kpost1 comb tile gA gB gC eA eB fA fB bid tid **
+  kpost1 #_ #_ comb #_ #_ #_ tile gA gB gC eA eB fA fB bid tid **
   (exists* x. gpu_pts_to_array (fst sh) #(1.0R /. (tile * tile)) x) **
   (exists* x. gpu_pts_to_array (fst (snd sh)) #(1.0R /. (tile * tile)) x) **
-  barrier_tok tile slA slB (fst sh) (fst (snd sh)) (2 * mshared) tid
+  barrier_tok tile slA slB (fst sh) (fst (snd sh)) (2 * SZ.v mshared) tid
 
 (* TODO: Find out where the time is going when checking this function,
 it feels a lot slower than the others. *)
@@ -195,9 +212,14 @@ fn kf
   (#et : Type0) {| scalar et |}
   (comb : binop et)
   (#mrows #mshared #mcols : SZ.t)
-  (#lA : mlayout (mrows   * tile) (mshared * tile))
-  (#lB : mlayout (mshared * tile) (mcols   * tile))
-  (#lC : mlayout (mrows   * tile) (mcols   * tile))
+  (#_ : squash (SZ.fits (SZ.v mrows   * SZ.v tile)))
+  (#_ : squash (SZ.fits (SZ.v mshared * SZ.v tile)))
+  (#_ : squash (SZ.fits (SZ.v mcols   * SZ.v tile)))
+  (#_ : squash (SZ.fits (SZ.v mrows   * SZ.v mcols)))
+  (#_ : squash (SZ.fits (2 * SZ.v mshared)))
+  (#lA : mlayout (mrows   *^ tile) (mshared *^ tile))
+  (#lB : mlayout (mshared *^ tile) (mcols   *^ tile))
+  (#lC : mlayout (mrows   *^ tile) (mcols   *^ tile))
   {| clayout lA, clayout lB, clayout lC |}
   (gA : gpu_matrix et lA)
   (gB : gpu_matrix et lB)
@@ -227,7 +249,7 @@ fn kf
   gpu_pts_to_ref ar1;
   gpu_pts_to_ref ar2;
 
-  unfold barrier_tok tile slA slB ar1 ar2 0 tid;
+  unfold barrier_tok tile slA slB ar1 ar2 0sz tid;
 
   M.gpu_matrix_abs' slA ar1;
   let sa1 = M.from_array slA ar1;
@@ -365,12 +387,15 @@ fn kf
   M.gpu_matrix_concr sa1; rewrite each M.core sa1 as ar1;
   M.gpu_matrix_concr sa2; rewrite each M.core sa2 as ar2;
 
-  fold barrier_tok tile slA slB ar1 ar2 (2 * mshared) tid;
+  fold barrier_tok tile slA slB ar1 ar2 (2sz *^ mshared) tid;
 
   rewrite each ar1 as fst sh;
   rewrite each ar2 as fst (snd sh);
   ()
 }
+
+unfold
+let szlt2 (x y : SZ.t{SZ.fits (SZ.v x * SZ.v y)}) = szlt (SZ.v (x *^ y))
 
 ghost
 fn setup
@@ -378,9 +403,14 @@ fn setup
   (#et : Type0) {| scalar et |}
   (comb : binop et)
   (#mrows #mshared #mcols : SZ.t)
-  (#lA : mlayout (mrows   * tile) (mshared * tile))
-  (#lB : mlayout (mshared * tile) (mcols   * tile))
-  (#lC : mlayout (mrows   * tile) (mcols   * tile))
+  (#_ : squash (SZ.fits (SZ.v mrows   * SZ.v tile)))
+  (#_ : squash (SZ.fits (SZ.v mshared * SZ.v tile)))
+  (#_ : squash (SZ.fits (SZ.v mcols   * SZ.v tile)))
+  (#_ : squash (SZ.fits (SZ.v mrows   * SZ.v mcols)))
+  (#_ : squash (SZ.fits (2 * SZ.v mshared)))
+  (#lA : mlayout (mrows   *^ tile) (mshared *^ tile))
+  (#lB : mlayout (mshared *^ tile) (mcols   *^ tile))
+  (#lC : mlayout (mrows   *^ tile) (mcols   *^ tile))
   {| clayout lA, clayout lB, clayout lC |}
   (gA : gpu_matrix et lA)
   (gB : gpu_matrix et lB)
@@ -393,8 +423,8 @@ fn setup
     (gB |-> Frac fB eB) **
     (gC |-> eC)
   ensures
-    (forall+ (bid : natlt2 mrows mcols)
-             (tid : natlt2 tile  tile).
+    (forall+ (bid : szlt (mrows *^ mcols))
+             (tid : szlt (tile  *^ tile)).
       kpre1 comb tile gA gB gC eA eB fA fB bid tid) **
     emp (* frame *)
 {
@@ -408,28 +438,33 @@ fn block_setup
   (#et : Type0) {| scalar et |}
   (comb : binop et)
   (#mrows #mshared #mcols : SZ.t)
-  (#lA : mlayout (mrows   * tile) (mshared * tile))
-  (#lB : mlayout (mshared * tile) (mcols   * tile))
-  (#lC : mlayout (mrows   * tile) (mcols   * tile))
+  (#_ : squash (SZ.fits (SZ.v mrows   * SZ.v tile)))
+  (#_ : squash (SZ.fits (SZ.v mshared * SZ.v tile)))
+  (#_ : squash (SZ.fits (SZ.v mcols   * SZ.v tile)))
+  (#_ : squash (SZ.fits (SZ.v mrows   * SZ.v mcols)))
+  (#_ : squash (SZ.fits (2 * SZ.v mshared)))
+  (#lA : mlayout (mrows   *^ tile) (mshared *^ tile))
+  (#lB : mlayout (mshared *^ tile) (mcols   *^ tile))
+  (#lC : mlayout (mrows   *^ tile) (mcols   *^ tile))
   {| clayout lA, clayout lB, clayout lC |}
   (gA : gpu_matrix et lA)
   (gB : gpu_matrix et lB)
   (gC : gpu_matrix et lC)
   (#fA #fB : perm)
-  (#eA : ematrix et (mrows * tile) (mshared * tile))
-  (#eB : ematrix et (mshared * tile) (mcols * tile))
-  (#eC : ematrix et (mrows * tile) (mcols * tile))
+  (#eA : ematrix et (mrows *^ tile) (mshared *^ tile))
+  (#eB : ematrix et (mshared *^ tile) (mcols *^ tile))
+  (#eC : ematrix et (mrows *^ tile) (mcols *^ tile))
   (sh : c_shmems (shmems_desc et tile))
-  (bid : natlt (mrows * mcols))
+  (bid : szlt (mrows *^ mcols))
   ()
   requires
     block_setup_tok (tile *^ tile) **
     live_c_shmems sh **
-    (forall+ (tid : natlt2 tile  tile).
+    (forall+ (tid : szlt2 tile  tile).
       kpre1 comb tile gA gB gC eA eB fA fB bid tid)
   ensures
     block_setup_tok (tile *^ tile) **
-    (forall+ (tid : natlt2 tile  tile).
+    (forall+ (tid : szlt2 tile  tile).
       kpre comb tile slA slB gA gB gC eA eB fA fB sh bid tid) **
     emp (* frame *)
 {
@@ -443,27 +478,32 @@ fn block_teardown
   (#et : Type0) {| scalar et |}
   (comb : binop et)
   (#mrows #mshared #mcols : SZ.t)
-  (#lA : mlayout (mrows   * tile) (mshared * tile))
-  (#lB : mlayout (mshared * tile) (mcols   * tile))
-  (#lC : mlayout (mrows   * tile) (mcols   * tile))
+  (#_ : squash (SZ.fits (SZ.v mrows   * SZ.v tile)))
+  (#_ : squash (SZ.fits (SZ.v mshared * SZ.v tile)))
+  (#_ : squash (SZ.fits (SZ.v mcols   * SZ.v tile)))
+  (#_ : squash (SZ.fits (SZ.v mrows   * SZ.v mcols)))
+  (#_ : squash (SZ.fits (2 * SZ.v mshared)))
+  (#lA : mlayout (mrows   *^ tile) (mshared *^ tile))
+  (#lB : mlayout (mshared *^ tile) (mcols   *^ tile))
+  (#lC : mlayout (mrows   *^ tile) (mcols   *^ tile))
   {| clayout lA, clayout lB, clayout lC |}
   (gA : gpu_matrix et lA)
   (gB : gpu_matrix et lB)
   (gC : gpu_matrix et lC)
   (#fA #fB : perm)
-  (#eA : ematrix et (mrows * tile) (mshared * tile))
-  (#eB : ematrix et (mshared * tile) (mcols * tile))
-  (#eC : ematrix et (mrows * tile) (mcols * tile))
+  (#eA : ematrix et (mrows *^ tile) (mshared *^ tile))
+  (#eB : ematrix et (mshared *^ tile) (mcols *^ tile))
+  (#eC : ematrix et (mrows *^ tile) (mcols *^ tile))
   (sh : c_shmems (shmems_desc et tile))
-  (bid : natlt (mrows * mcols))
+  (bid : szlt (mrows *^ mcols))
   ()
   requires
-    (forall+ (tid : natlt2 tile  tile).
+    (forall+ (tid : szlt2 tile  tile).
       kpost comb tile slA slB gA gB gC eA eB fA fB sh bid tid) **
     emp (* frame *)
   ensures
     live_c_shmems sh **
-    (forall+ (tid : natlt2 tile  tile).
+    (forall+ (tid : szlt2 tile  tile).
       kpost1 comb tile gA gB gC eA eB fA fB bid tid)
 {
   admit();
@@ -475,21 +515,26 @@ fn teardown
   (#et : Type0) {| scalar et |}
   (comb : binop et)
   (#mrows #mshared #mcols : SZ.t)
-  (#lA : mlayout (mrows   * tile) (mshared * tile))
-  (#lB : mlayout (mshared * tile) (mcols   * tile))
-  (#lC : mlayout (mrows   * tile) (mcols   * tile))
+  (#_ : squash (SZ.fits (SZ.v mrows   * SZ.v tile)))
+  (#_ : squash (SZ.fits (SZ.v mshared * SZ.v tile)))
+  (#_ : squash (SZ.fits (SZ.v mcols   * SZ.v tile)))
+  (#_ : squash (SZ.fits (SZ.v mrows   * SZ.v mcols)))
+  (#_ : squash (SZ.fits (2 * SZ.v mshared)))
+  (#lA : mlayout (mrows   *^ tile) (mshared *^ tile))
+  (#lB : mlayout (mshared *^ tile) (mcols   *^ tile))
+  (#lC : mlayout (mrows   *^ tile) (mcols   *^ tile))
   {| clayout lA, clayout lB, clayout lC |}
   (gA : gpu_matrix et lA)
   (gB : gpu_matrix et lB)
   (gC : gpu_matrix et lC)
   (#fA #fB : perm)
-  (#eA : ematrix et (mrows * tile) (mshared * tile))
-  (#eB : ematrix et (mshared * tile) (mcols * tile))
-  (#eC : ematrix et (mrows * tile) (mcols * tile))
+  (#eA : ematrix et (mrows *^ tile) (mshared *^ tile))
+  (#eB : ematrix et (mshared *^ tile) (mcols *^ tile))
+  (#eC : ematrix et (mrows *^ tile) (mcols *^ tile))
   ()
   requires
-    (forall+ (bid : natlt2 mrows mcols)
-             (tid : natlt2 tile  tile).
+    (forall+ (bid : szlt2 mrows mcols)
+             (tid : szlt2 tile  tile).
       kpost1 comb tile gA gB gC eA eB fA fB bid tid) **
     emp (* frame *)
   ensures
@@ -500,25 +545,32 @@ fn teardown
   admit();
 }
 
+#set-options "--print_implicits --debug SMTFail,ExplainRel"
+
 inline_for_extraction noextract
 let mk_kernel
   (tile : valid_tile)
   (slA slB : full_mlayout tile tile) // shmem layouts
   {| clayout slA, clayout slB |}
-  (#et : Type0) {| scalar et |}
+  (#et : Type0) {| s_et : scalar et |}
   (comb : binop et)
   (#mrows #mshared #mcols : szp)
-  (#lA : mlayout (mrows   * tile) (mshared * tile))
-  (#lB : mlayout (mshared * tile) (mcols   * tile))
-  (#lC : mlayout (mrows   * tile) (mcols   * tile))
+  (#_ : squash (SZ.fits (SZ.v mrows   * SZ.v tile)))
+  (#_ : squash (SZ.fits (SZ.v mshared * SZ.v tile)))
+  (#_ : squash (SZ.fits (SZ.v mcols   * SZ.v tile)))
+  (#_ : squash (SZ.fits (SZ.v mrows   * SZ.v mcols)))
+  (#_ : squash (SZ.fits (2 * SZ.v mshared)))
+  (#lA : mlayout (mrows   *^ tile) (mshared *^ tile))
+  (#lB : mlayout (mshared *^ tile) (mcols   *^ tile))
+  (#lC : mlayout (mrows   *^ tile) (mcols   *^ tile))
   {| clayout lA, clayout lB, clayout lC |}
   (gA : gpu_matrix et lA)
   (gB : gpu_matrix et lB)
   (gC : gpu_matrix et lC)
   (#fA #fB : perm)
-  (#eA : ematrix et (mrows * tile) (mshared * tile))
-  (#eB : ematrix et (mshared * tile) (mcols * tile))
-  (#eC : ematrix et (mrows * tile) (mcols * tile))
+  (#eA : ematrix et (mrows *^ tile) (mshared *^ tile))
+  (#eB : ematrix et (mshared *^ tile) (mcols *^ tile))
+  (#eC : ematrix et (mrows *^ tile) (mcols *^ tile))
   (_ : squash (mrows * mcols <= max_blocks
                /\ tile * tile <= max_threads))
   : kernel_desc
@@ -531,9 +583,9 @@ let mk_kernel
   shmems_desc = shmems_desc et tile;
 
   frame = emp;
-  block_pre  = (fun bid -> forall+ (tid : natlt2 tile tile). kpre1  comb tile gA gB gC eA eB fA fB bid tid);
-  block_post = (fun bid -> forall+ (tid : natlt2 tile tile). kpost1 comb tile gA gB gC eA eB fA fB bid tid);
-  setup      = setup    tile comb gA gB gC;
+  block_pre  = (fun bid -> forall+ (tid : szlt (tile *^ tile)). kpre1  comb tile gA gB gC eA eB fA fB bid tid);
+  block_post = (fun bid -> forall+ (tid : szlt (tile *^ tile)). kpost1 comb tile gA gB gC eA eB fA fB bid tid);
+  setup      = setup    tile #et #s_et comb #mrows #mshared #mcols #() #() #() #() #() #lA #lB #lC gA gB gC #fA #fB #eA #eB #eC;
   teardown   = teardown tile comb gA gB gC;
 
   block_frame    = (fun _ar _bid -> emp);
@@ -552,25 +604,30 @@ fn mmcomb_gpu
   (#et : Type0) {| scalar et |}
   (comb : binop et)
   (#mrows #mshared #mcols : szp)
-  (lA : mlayout (mrows   * tile) (mshared * tile))
-  (lB : mlayout (mshared * tile) (mcols   * tile))
-  (lC : mlayout (mrows   * tile) (mcols   * tile))
+  (#_ : squash (SZ.fits (SZ.v mrows   * SZ.v tile)))
+  (#_ : squash (SZ.fits (SZ.v mshared * SZ.v tile)))
+  (#_ : squash (SZ.fits (SZ.v mcols   * SZ.v tile)))
+  (#_ : squash (SZ.fits (SZ.v mrows   * SZ.v mcols)))
+  (#_ : squash (SZ.fits (2 * SZ.v mshared)))
+  (lA : mlayout (mrows   *^ tile) (mshared *^ tile))
+  (lB : mlayout (mshared *^ tile) (mcols   *^ tile))
+  (lC : mlayout (mrows   *^ tile) (mcols   *^ tile))
   {| clayout lA, clayout lB, clayout lC |}
   (gA : gpu_matrix et lA)
   (#fA : perm)
   (gB : gpu_matrix et lB)
   (#fB : perm)
   (gC : gpu_matrix et lC)
-  (#eA : ematrix et (mrows * tile) (mshared * tile))
-  (#eB : ematrix et (mshared * tile) (mcols * tile))
-  (#eC : ematrix et (mrows * tile) (mcols * tile))
+  (#eA : ematrix et (mrows *^ tile) (mshared *^ tile))
+  (#eB : ematrix et (mshared *^ tile) (mcols *^ tile))
+  (#eC : ematrix et (mrows *^ tile) (mcols *^ tile))
   preserves
     cpu **
     (gA |-> Frac fA eA) **
     (gB |-> Frac fB eB)
   requires
-    pure (mrows * mcols <= max_blocks) **
-    pure (tile * tile <= max_threads) **
+    pure (mrows *^ mcols <= max_blocks) **
+    pure (tile *^ tile <= max_threads) **
     (gC |-> eC)
   ensures
     gC |-> MS.mmcomb comb eC eA eB
