src/lib/kuiper/Kuiper.SizeT.fsti
@@ -97,3 +97,4 @@ let lem_sdivup (x:sz) (y:szp{SZ.fits (x+y)})
   : Lemma (SZ.v (sdivup x y) == divup (SZ.v x) (SZ.v y))
           [SMTPat (sdivup x y)]
   = ()
+
